reals/fast/CRsin.v
@@ -23,45 +23,522 @@ Require Import CRAlternatingSum.
 Require Export CRArith.
 Require Import CRIR.
 Require Import Qpower.
+Require Import Qordfield.
+Require Import ModulusDerivative.
+Require Import ContinuousCorrect.
+Require Import Qmetric.
+Require Import PowerSeries.
+Require Import SinCos.
+Require Import Ndigits.
 Require Import CornTac.
 
 Set Implicit Arguments.
 
-Opaque CR.
-
 Open Local Scope Q_scope.
+Open Local Scope uc_scope.
 
-Section CosSeries.
+Opaque inj_Q CR Qmin Qmax.
+
+Section SinSeries.
 Variable a:Q.
 
-Definition cosSequence := (mult_Streams (everyOther recip_factorials) (powers (a^2))).
+Definition sinSequence := (mult_Streams (everyOther (tl recip_factorials)) (powers_help (a^2) a)).
 
-Lemma Str_nth_cosSequence : forall n, (Str_nth n cosSequence == (1#P_of_succ_nat (pred (fac (2*n))))*a^(2*n)%nat)%Q.
+Lemma Str_nth_sinSequence : forall n, (Str_nth n sinSequence == (1#P_of_succ_nat (pred (fac (1+2*n))))*a^(1+2*n)%nat)%Q.
 Proof.
 intros n.
-unfold cosSequence.
+unfold sinSequence.
 unfold mult_Streams.
 rewrite Str_nth_zipWith.
 rewrite Str_nth_everyOther.
+change (tl recip_factorials) with (Str_nth_tl 1 recip_factorials).
+rewrite Str_nth_plus.
+rewrite plus_comm.
 rewrite Str_nth_recip_factorials.
-rewrite Str_nth_powers.
-rewrite Qpower
+rewrite Str_nth_powers_help.
+rewrite <- Qpower_mult.
+destruct (Qeq_dec a 0).
+ rewrite q.
+ rewrite (Qpower_0 (1+2*n)%nat);[|ring].
+ discriminate.
+rewrite inj_plus.
+rewrite Qpower_plus.
+ assumption.
+rewrite inj_mult.
 reflexivity.
 Qed.
 
-Hypothesis Ha: -(1) <= a <= 1.
+Hypothesis Ha: 0 <= a <= 1.
 
-Lemma cosSequence_dnn : DecreasingNonNegative cosSequence.
+Lemma square_zero_one : 0 <= a^2 <= 1.
 Proof.
-apply recip_factorials_dnn.
-apply powers_dnn.
+split.
+ replace RHS with ((1*a)*a) by ring.
+ rapply (sqr_nonneg _ a).
+rewrite Qle_minus_iff.
+replace RHS with ((1-a)*(1+a)) by ring.
+destruct Ha as [Ha0 Ha1].
+rsapply mult_resp_nonneg;
+ [unfold Qminus|replace RHS with (a + - (-(1))) by ring];
+ rewrite <- Qle_minus_iff;
+ try assumption.
+apply Qle_trans with 0.
+ discriminate.
 assumption.
 Qed.
 
-Lemma expSequence_zl : Limit expSequence 0.
+Lemma sinSequence_dnn : DecreasingNonNegative sinSequence.
 Proof.
-rapply mult_Streams_zl.
-apply recip_factorials_zl.
-apply powers_nbz.
-assumption.
+rapply mult_Streams_dnn.
+ apply everyOther_dnn.
+ apply dnn_tl.
+ apply recip_factorials_dnn.
+apply powers_help_dnn.
+ apply square_zero_one; assumption.
+destruct Ha; assumption.
+Qed.
+
+Lemma sinSequence_zl : Limit sinSequence 0.
+Proof.
+unfold sinSequence.
+apply mult_Streams_zl with (1#1)%Qpos.
+ apply everyOther_zl.
+ rapply Limit_tl.
+ apply recip_factorials_zl.
+apply powers_help_nbz; try
+ apply square_zero_one; assumption.
 Defined.
+
+End SinSeries.
+
+Definition rational_sin_small_pos (a:Q) (p: 0 <= a <= 1) : CR := 
+ InfiniteAlternatingSum (sinSequence_dnn p) (sinSequence_zl p).
+
+Lemma rational_sin_small_pos_correct : forall (a:Q) Ha,
+ (@rational_sin_small_pos a Ha == IRasCR (Sin (inj_Q IR a)))%CR.
+Proof.
+intros a Ha.
+unfold rational_sin_small_pos.
+simpl.
+generalize (fun_series_conv_imp_conv (inj_Q IR a) (inj_Q IR a)
+         (leEq_reflexive IR (inj_Q IR a)) sin_ps
+         (sin_conv (inj_Q IR a) (inj_Q IR a) (leEq_reflexive IR (inj_Q IR a))
+            (compact_single_iprop realline (inj_Q IR a) CI)) (inj_Q IR a)
+         (compact_single_prop (inj_Q IR a))
+         (fun_series_inc_IR realline sin_ps sin_conv (inj_Q IR a) CI)).
+intros H.
+rewrite InfiniteAlternatingSum_correct'.
+apply IRasCR_wd.
+unfold series_sum.
+apply Lim_seq_eq_Lim_subseq with (fun n => 2*n)%nat.
+  intros; omega.
+ intros n; exists (S n); omega.
+intros n.
+induction n.
+ apply eq_reflexive.
+replace (2*(S n))%nat with (S (S (2*n)))%nat by omega.
+set (n':=(2*n)%nat) in *.
+simpl in *.
+rstepr (seq_part_sum
+  (fun n0 : nat =>
+   (sin_seq n0[/]nring (R:=IR) (fac n0)[//]nring_fac_ap_zero IR n0)[*]
+   nexp IR n0 (inj_Q IR a[-]Zero)) n'[+](
+(sin_seq n'[/]nring (R:=IR) (fac n')[//]nring_fac_ap_zero IR n')[*]
+nexp IR n' (inj_Q IR a[-]Zero)[+]
+(sin_seq (S n')[/]nring (R:=IR) (fac n' + n' * fac n')[//]
+ nring_fac_ap_zero IR (S n'))[*]
+(nexp IR n' (inj_Q IR a[-]Zero)[*](inj_Q IR a[-]Zero)))).
+apply bin_op_wd_unfolded.
+ assumption.
+rstepl (Zero[+]inj_Q IR ((- (1)) ^ n * Str_nth n (sinSequence a))).
+unfold sin_seq.
+apply bin_op_wd_unfolded.
+ destruct (even_or_odd_plus n') as [m [Hm|Hm]]; simpl.
+   rational.
+ elim (not_even_and_odd n').
+  rapply (even_mult_l 2 n).
+  repeat constructor.
+ rewrite Hm.
+ constructor.
+ replace (m + m)%nat with (2*m)%nat by omega.
+ apply (even_mult_l 2 m).
+ repeat constructor.
+destruct (even_or_odd_plus (S n')) as [m [Hm|Hm]]; simpl.
+ elim (not_even_and_odd (S n')).
+  rewrite Hm.
+  replace (m + m)%nat with (2*m)%nat by omega.
+  rapply (even_mult_l 2 m).
+  repeat constructor.
+ constructor.
+ apply (even_mult_l 2 n).
+ repeat constructor.
+inversion Hm.
+unfold n' in H1.
+replace m with n by omega.
+clear Hm H1.
+stepl ((inj_Q IR ((-(1))^n))[*](inj_Q IR (Str_nth n (sinSequence a)))) by
+ (apply eq_symmetric; apply inj_Q_mult).
+change (inj_Q IR ((- (1)) ^ n)[*]inj_Q IR (Str_nth n (sinSequence a))[=]
+(nexp IR n [--]One[/]nring (R:=IR) (fac (S n'))[//]nring_fac_ap_zero IR (S n'))[*]
+(nexp IR (S n') (inj_Q IR a[-]Zero))).
+rstepr ((nexp IR n [--]One[*](nexp IR (S n') (inj_Q IR a[-]Zero)[/]nring (R:=IR) (fac (S n'))[//]
+ nring_fac_ap_zero IR (S n')))).
+apply mult_wd.
+ stepr ((inj_Q IR (-(1)))[^]n).
+  apply inj_Q_power.
+ rapply nexp_wd.
+ stepr ([--](inj_Q IR 1)).
+  apply inj_Q_min.
+ apply un_op_wd_unfolded.
+ rstepr (nring 1:IR).
+ apply (inj_Q_nring IR 1).
+stepr (inj_Q IR ((1/P_of_succ_nat (pred (fac (1+2*n))))*a^(1+2*n)%nat)).
+ apply inj_Q_wd.
+ simpl.
+ rewrite Str_nth_sinSequence.
+ rewrite Qmake_Qdiv.
+ reflexivity.
+rstepr ((nring 1[/]nring (R:=IR) (fac (S n'))[//]
+ nring_fac_ap_zero IR (S n'))[*](nexp IR (S n') (inj_Q IR a[-]Zero))).
+change (1+2*n)%nat with (S n').
+stepr ((inj_Q IR (1 / P_of_succ_nat (pred (fac (S n'))))[*](inj_Q IR (a^S n')))).
+ apply inj_Q_mult.
+apply mult_wd.
+ rewrite <- POS_anti_convert.
+ assert (X:inj_Q IR (inject_Z (Z_of_nat (S (pred (fac (S n'))))))[#]Zero).
+  stepr (inj_Q IR Zero).
+   assert (inject_Z (Z_of_nat (S (pred (fac (S n')))))[#]Zero).
+    discriminate.
+   destruct (ap_imp_less _ _ _ X).
+    apply less_imp_ap.
+    apply inj_Q_less.
+    assumption.
+   apply Greater_imp_ap.
+   apply inj_Q_less.
+   assumption.
+  apply (inj_Q_nring IR 0).
+ stepr ((inj_Q IR 1)[/](inj_Q IR (inject_Z (Z_of_nat (S (pred (fac (S n')))))))[//]X).
+  apply inj_Q_div.
+ apply div_wd.
+  apply (inj_Q_nring IR 1).
+ stepl (inj_Q IR (nring (fac (S n')))).
+  apply inj_Q_nring.
+ assert (Y:=nat_fac_gtzero (S n')).
+ apply inj_Q_wd.
+ stepr ((fac (S n')):Q).
+  clear - n'.
+  induction (fac (S n')).
+   simpl; reflexivity.
+  rewrite inj_S.
+  unfold Zsucc.
+  simpl in *.
+  rewrite IHn0.
+  rewrite injz_plus.
+  reflexivity.
+ destruct (fac (S n')).
+  elimtype False; auto with *.
+ simpl; reflexivity.
+stepr ((inj_Q IR a)[^](S n')).
+ apply inj_Q_power.
+change (inj_Q IR a[^]S n'[=](inj_Q IR a[-]Zero)[^]S n').
+apply nexp_wd.
+rational.
+Qed.
+
+Section Sin_Poly.
+
+Definition sin_poly_fun (x:Q) :Q := x*(3 - 4*x*x).
+
+Lemma sin_poly_fun_correct : forall (q:Q),
+ inj_Q IR (sin_poly_fun q)[=]Three[*]inj_Q IR q[-]Four[*](inj_Q IR q[^]3).
+Proof.
+intros q.
+unfold sin_poly_fun.
+stepr (inj_Q IR (3*q-4*q^3)).
+ apply inj_Q_wd.
+ simpl; ring.
+stepr (inj_Q IR (Three[*]q)[-]inj_Q IR (Four[*]q ^ 3))%Q.
+ apply inj_Q_minus.
+apply cg_minus_wd.
+ stepr (inj_Q IR Three[*]inj_Q IR q).
+  apply inj_Q_mult.
+ apply mult_wdl.
+ apply (inj_Q_nring IR 3).
+stepr (inj_Q IR Four[*]inj_Q IR (q^3)).
+ apply inj_Q_mult.
+apply mult_wd.
+ apply (inj_Q_nring IR 4).
+apply (inj_Q_power IR q 3).
+Qed.
+
+Definition sin_poly_modulus (e:Qpos) := Qpos2QposInf (e/(9#1)).
+
+Let X:((-(1))<1)%Q.
+constructor.
+Qed.
+
+Let D : Derivative (clcr (inj_Q IR (-(1))) (inj_Q IR (1:Q))) (inj_Q_less _ _ _ X) ((Three:IR){**}FId{-}(Four:IR){**}FId{^}3)
+ ((Three:IR){**}[-C-](One:IR){-}(Four:IR){**}((nring 3){**}([-C-]One{*}FId{^}2))).
+apply Derivative_minus.
+ apply Derivative_scal.
+ apply Derivative_id.
+apply Derivative_scal.
+apply Derivative_nth.
+apply Derivative_id.
+Qed.
+
+Lemma sin_poly_prf : is_UniformlyContinuousFunction (fun x => sin_poly_fun (QboundAbs (1#1) x)) sin_poly_modulus.
+Proof.
+rapply (is_UniformlyContinuousD_Q (Some (-(1))%Q) (Some (1:Q)) X _ _ D sin_poly_fun).
+ simpl; intros q _ _.
+ rapply sin_poly_fun_correct.
+simpl; intros x _ [Hx0 Hx1].
+stepr (Nine:IR) by (apply eq_symmetric; apply (inj_Q_nring IR 9)).
+stepl (ABSIR (Three[-]Twelve[*]x[*]x)) by (apply AbsIR_wd; rational).
+apply AbsSmall_imp_AbsIR.
+split.
+ apply shift_zero_leEq_minus'.
+ rstepr (Twelve[*]((nring 1)[-]x)[*](x[-][--](nring 1))).
+ repeat apply mult_resp_nonneg.
+   apply (nring_nonneg IR 12).
+  apply shift_zero_leEq_minus.
+  stepr (inj_Q IR (nring 1)) by apply inj_Q_nring.
+  assumption.
+ apply shift_zero_leEq_minus.
+ stepl (inj_Q IR (-(1))).
+  assumption.
+ stepr ([--](inj_Q IR 1)).
+  apply inj_Q_min.
+ rapply un_op_wd_unfolded.
+ apply (inj_Q_nring IR 1).
+ rstepr (Nine[-]Zero:IR).
+apply minus_resp_leEq_both.
+ apply nring_leEq.
+ omega.
+rstepr (Twelve[*]x[^]2).
+apply mult_resp_nonneg.
+ apply (nring_leEq  IR 0 12).
+ omega.
+apply sqr_nonneg.
+Qed.
+
+Definition sin_poly_uc : Q_as_MetricSpace --> Q_as_MetricSpace := 
+Build_UniformlyContinuousFunction sin_poly_prf.
+
+Definition sin_poly : CR --> CR := Cmap QPrelengthSpace sin_poly_uc.
+
+Lemma sin_poly_correct : forall x, AbsSmall (inj_Q IR (1)) x -> (IRasCR (Three[*]x[-]Four[*]x[^]3)==sin_poly (IRasCR x))%CR.
+Proof.
+intros x Hx.
+assert (Y:Continuous (clcr (inj_Q IR (-(1))) (inj_Q IR (1:Q))) ((Three:IR){**}FId{-}(Four:IR){**}FId{^}3)).
+ eapply Derivative_imp_Continuous.
+ apply D.
+rapply (ContinuousCorrect (I:=(clcr (inj_Q IR (-(1))) (inj_Q IR (1:Q)))) (inj_Q_less _ _ _ X) Y);
+ [|repeat constructor|].
+ intros q Hq Hq0.
+ transitivity (IRasCR (inj_Q IR (sin_poly_fun q)));[|apply IRasCR_wd; rapply sin_poly_fun_correct].
+ simpl.
+ change (' q)%CR with (Cunit_fun _ q).
+ rewrite MonadLaw3.
+ rewrite IR_inj_Q_as_CR.
+ rewrite CReq_Qeq.
+ simpl.
+ unfold sin_poly_fun.
+ setoid_replace (Qmax (- (1 # 1)%Qpos) (Qmin (1 # 1)%Qpos q)) with q.
+  reflexivity.
+ setoid_replace (Qmin (1 # 1)%Qpos q) with q.
+  rewrite <- Qle_max_r.
+  apply leEq_inj_Q with IR.
+  destruct Hq0; assumption.
+ rewrite <- Qle_min_r.
+ apply leEq_inj_Q with IR.
+ destruct Hq0; assumption.
+destruct Hx; split;[stepl [--](inj_Q IR (1:Q)) by apply eq_symmetric; apply inj_Q_min|];assumption.
+Qed.
+
+Lemma Sin_triple_angle : forall x, (Sin(Three[*]x)[=]Three[*]Sin x[-]Four[*]Sin x[^]3).
+Proof.
+intros x.
+assert (H:Three[*]x[=]x[+]x[+]x) by rational.
+csetoid_rewrite H.
+csetoid_rewrite (Sin_plus (x[+]x) x).
+csetoid_rewrite (Sin_plus x x).
+csetoid_rewrite (Cos_plus x x).
+set (sx:=Sin x).
+set (cx:=Cos x).
+rstepl ((cx[^]2)[*](Three[*]sx)[-]sx[^]3).
+unfold cg_minus.
+csetoid_replace (cx[^]2) (One[-]sx[^]2).
+ rational.
+apply cg_inv_unique_2.
+rstepl ((cx[^]2[+]sx[^]2)[-]One).
+apply x_minus_x.
+rapply FFT.
+Qed.
+
+Lemma shrink_by_three : forall n a, 0 <= a <= (3^(S n))%Z -> 0 <= a/3 <= (3^n)%Z.
+Proof.
+intros n a [H0 H1].
+split.
+ rapply mult_resp_nonneg.
+  assumption.
+ discriminate.
+apply Qmult_lt_0_le_reg_r with 3.
+ constructor.
+rewrite Zpower_Qpower.
+ auto with *.
+rewrite (inj_S n) in H1.
+replace RHS with (3%positive^n*3^1) by ring.
+rewrite <- Qpower_plus.
+ discriminate.
+replace LHS with a by (field; discriminate).
+rewrite Zpower_Qpower in H1.
+ assumption.
+auto with *.
+Qed.
+
+Fixpoint rational_sin_pos_bounded (n:nat) (a:Q) : 0 <= a <= (3^n)%Z -> CR :=
+match n return 0 <= a <= (3^n)%Z -> CR with 
+| O => @rational_sin_small_pos a
+| S n' => 
+  match (Qlt_le_dec 1 a) with
+  | left _ => fun H => sin_poly (rational_sin_pos_bounded n' (shrink_by_three n' H))
+  | right H' => fun H => rational_sin_small_pos (conj (proj1 H) H')
+  end
+end.
+
+Lemma rational_sin_pos_bounded_correct :  forall n (a:Q) Ha,
+ (@rational_sin_pos_bounded n a Ha == IRasCR (Sin (inj_Q IR a)))%CR.
+Proof.
+induction n.
+ rapply rational_sin_small_pos_correct.
+intros a Ha.
+unfold rational_sin_pos_bounded; fold rational_sin_pos_bounded.
+destruct (Qlt_le_dec 1 a);[|rapply rational_sin_small_pos_correct].
+rewrite IHn.
+rewrite <- sin_poly_correct.
+ apply AbsIR_imp_AbsSmall.
+ stepr (nring 1:IR) by (apply eq_symmetric; apply (inj_Q_nring IR 1)).
+ rstepr (One:IR).
+ apply AbsIR_Sin_leEq_One.
+apply IRasCR_wd.
+stepl (Sin (inj_Q IR (a/3*3))).
+ apply Sin_wd.
+ apply inj_Q_wd.
+ simpl; field; discriminate.
+generalize (a/3).
+intros b; clear -b.
+stepr (Sin (Three[*](inj_Q IR b))).
+ apply Sin_wd.
+ stepr ((inj_Q IR b)[*](inj_Q IR (3:Q))).
+  apply inj_Q_mult.
+ csetoid_replace (inj_Q IR (3:Q)) (Three:IR).
+  rational.
+ apply (inj_Q_nring IR 3).
+apply Sin_triple_angle.
+Qed.
+
+End Sin_Poly.
+
+Lemma power3bound : forall q, (q <= (3^(Z_of_nat (let (n,_):= q in match n with Zpos p => Psize p | _ => O end)))%Z).
+intros [[|n|n] d]; try discriminate.
+unfold Qle.
+simpl.
+Open Scope Z_scope.
+rewrite Zpos_mult_morphism.
+apply Zmult_le_compat; auto with *.
+clear - n.
+apply Zle_trans with (two_p (Zsucc (log_inf n))-1)%Z.
+ rewrite <- Zle_plus_swap.
+ apply Zlt_succ_le.
+ change (n+1) with (Zsucc n).
+ apply Zsucc_lt_compat.
+ destruct (log_inf_correct2 n).
+ assumption.
+replace (Zsucc (log_inf n)) with (Z_of_nat (Psize n)).
+ apply Zle_trans with (two_p (Psize n)).
+  auto with *.
+ induction (Psize n); auto with *.
+ rewrite inj_S.
+ simpl.
+ unfold Zsucc.
+ rewrite two_p_is_exp; auto with *.
+ change (two_p 1) with 2.
+ rewrite Zpower_exp; auto with *.
+ change (3^1) with 3.
+ apply Zmult_le_compat; auto with *.
+ induction (Z_of_nat n0); auto with *.
+induction n; auto with *; simpl; rewrite <- IHn;
+ rewrite <- POS_anti_convert; rewrite inj_S; reflexivity.
+Close Scope Z_scope.
+Qed.
+
+Definition rational_sin_pos (a:Q) (Ha:0 <= a) : CR :=
+ @rational_sin_pos_bounded _ a (conj Ha (power3bound a)).
+
+Lemma rational_sin_pos_correct : forall (a:Q) Ha,
+ (@rational_sin_pos a Ha == IRasCR (Sin (inj_Q IR a)))%CR.
+Proof.
+intros; rapply rational_sin_pos_bounded_correct.
+Qed.
+
+Definition rational_sin (a:Q) : CR :=
+match (Qle_total 0 a) with
+| left H => rational_sin_pos H
+| right H => (-rational_sin_pos (Qopp_le_compat _ _ H))%CR
+end.
+
+Lemma rational_sin_correct : forall (a:Q),
+ (@rational_sin a == IRasCR (Sin (inj_Q IR a)))%CR.
+Proof.
+intros a.
+unfold rational_sin.
+destruct (Qle_total 0 a).
+ apply rational_sin_pos_correct.
+rewrite rational_sin_pos_correct.
+rewrite <- IR_opp_as_CR.
+apply IRasCR_wd.
+csetoid_rewrite_rev (Sin_inv (inj_Q IR (-a))).
+apply Sin_wd.
+csetoid_rewrite_rev (inj_Q_min IR (-a)).
+apply inj_Q_wd.
+simpl.
+ring.
+Qed.
+
+Definition sin_uc_prf : is_UniformlyContinuousFunction rational_sin Qpos2QposInf.
+Proof.
+apply (is_UniformlyContinuousFunction_wd) with (fun x => rational_sin x) (modulusD (1#1)).
+  reflexivity.
+ intros x.
+ simpl.
+ autorewrite with QposElim.
+ change (/1) with 1.
+ replace RHS with (x:Q) by ring.
+ apply Qle_refl.
+rapply (is_UniformlyContinuousD None None I Sine Cosine (Derivative_Sin CI) rational_sin).
+ intros q [] _.
+ rapply rational_sin_correct.
+intros x [] _.
+stepr (One:IR).
+ rapply AbsIR_Cos_leEq_One.
+rstepl (nring 1:IR).
+apply eq_symmetric.
+rapply (inj_Q_nring IR 1).
+Qed.
+
+Definition sin_uc : Q_as_MetricSpace --> CR := 
+Build_UniformlyContinuousFunction sin_uc_prf.
+
+Definition sin : CR --> CR := Cbind QPrelengthSpace sin_uc.
+
+Lemma sin_correct : forall x,
+ (IRasCR (Sin x) == sin (IRasCR x))%CR.
+Proof.
+intros x.
+rapply (ContinuousCorrect (CI:proper realline));
+ [apply Continuous_Sin | | constructor].
+intros q [] _.
+transitivity (rational_sin q);[|rapply rational_sin_correct].
+rapply BindLaw1.
+Qed.
